P1.fsti
@@ -15,14 +15,14 @@ module Spec = Trees
 
 (**** Stateful operations on generic trees *)
 /// Appends value [v] at the leftmost leaf of the tree that [ptr] points to.
-(*val append_left (#a: Type0) (ptr: t a) (v: a)
+val append_left (#a: Type0) (ptr: t a) (v: a)
     : Steel (t a)
       (linked_tree ptr)
       (fun ptr' ->  linked_tree ptr')
       (requires (fun h0 -> True))
       (ensures (fun h0 ptr' h1 -> v_linked_tree ptr' h1 == Spec.append_left (v_linked_tree ptr h0) v))
-*)
-(*)
+
+
 /// Appends value [v] at the rightmost leaf of the tree that [ptr] points to.
 val append_right (#a: Type0) (ptr: t a) (v: a)
     : Steel (t a)
@@ -32,7 +32,7 @@ val append_right (#a: Type0) (ptr: t a) (v: a)
       (ensures (fun h0 ptr' h1 ->
         v_linked_tree ptr' h1 == Spec.append_right (v_linked_tree ptr h0) v
       ))
-
+(*)
 /// Returns the height of the tree that [ptr] points to
 val height (#a: Type0) (ptr: t a)
     : Steel nat (linked_tree ptr) (fun _ -> linked_tree ptr)
